Flapjack/Test/CompilerParity.lean
@@ -132,6 +132,7 @@ import Flapjack.Test.CompileToCrepeParity
 import Flapjack.Test.CompileProgParity
 import Flapjack.Test.PanSimpParity
 import Flapjack.Test.PanProgramSimpParity
+import Flapjack.Test.PanValueWfParity
 import Flapjack.Test.PanGlobalsSemanticsParity
 import Flapjack.Test.PanSimpOthersParity
 import Flapjack.Test.CrepProgIfParity
